Strata/Languages/Boogie/Examples/DDMAxiomsExtraction.lean
@@ -239,7 +239,7 @@ info: #[{ name := { dialect := "Boogie", name := "command_typedecl" },
 /--
 info: [Lambda.LExpr.quant
    (Lambda.QuantifierKind.all)
-   (some (Lambda.LMonoTy.tcons "Map" [Lambda.LMonoTy.ftvar "k", Lambda.LMonoTy.ftvar "v"]))
+   (some (Lambda.LMonoTy.tcons "Map" [Lambda.LMonoTy.ftvar "k", Lambda.LMonoTy.ftvar "v"] ()))
    (Lambda.LExpr.bvar 0)
    (Lambda.LExpr.quant
      (Lambda.QuantifierKind.all)
@@ -256,8 +256,9 @@ info: [Lambda.LExpr.quant
                u:select
                (some (Lambda.LMonoTy.tcons
                   "arrow"
-                  [Lambda.LMonoTy.tcons "Map" [Lambda.LMonoTy.ftvar "k", Lambda.LMonoTy.ftvar "v"],
-                   Lambda.LMonoTy.tcons "arrow" [Lambda.LMonoTy.ftvar "k", Lambda.LMonoTy.ftvar "v"]])))
+                  [Lambda.LMonoTy.tcons "Map" [Lambda.LMonoTy.ftvar "k", Lambda.LMonoTy.ftvar "v"] (),
+                   Lambda.LMonoTy.tcons "arrow" [Lambda.LMonoTy.ftvar "k", Lambda.LMonoTy.ftvar "v"] ()]
+                  ())))
              (Lambda.LExpr.app
                (Lambda.LExpr.app
                  (Lambda.LExpr.app
@@ -265,14 +266,17 @@ info: [Lambda.LExpr.quant
                      u:update
                      (some (Lambda.LMonoTy.tcons
                         "arrow"
-                        [Lambda.LMonoTy.tcons "Map" [Lambda.LMonoTy.ftvar "k", Lambda.LMonoTy.ftvar "v"],
+                        [Lambda.LMonoTy.tcons "Map" [Lambda.LMonoTy.ftvar "k", Lambda.LMonoTy.ftvar "v"] (),
                          Lambda.LMonoTy.tcons
                            "arrow"
                            [Lambda.LMonoTy.ftvar "k",
                             Lambda.LMonoTy.tcons
                               "arrow"
                               [Lambda.LMonoTy.ftvar "v",
-                               Lambda.LMonoTy.tcons "Map" [Lambda.LMonoTy.ftvar "k", Lambda.LMonoTy.ftvar "v"]]]])))
+                               Lambda.LMonoTy.tcons "Map" [Lambda.LMonoTy.ftvar "k", Lambda.LMonoTy.ftvar "v"] ()]
+                              ()]
+                           ()]
+                        ())))
                    (Lambda.LExpr.bvar 2))
                  (Lambda.LExpr.bvar 1))
                (Lambda.LExpr.bvar 0)))
@@ -280,7 +284,7 @@ info: [Lambda.LExpr.quant
          (Lambda.LExpr.bvar 0)))),
  Lambda.LExpr.quant
    (Lambda.QuantifierKind.all)
-   (some (Lambda.LMonoTy.tcons "Map" [Lambda.LMonoTy.ftvar "k", Lambda.LMonoTy.ftvar "v"]))
+   (some (Lambda.LMonoTy.tcons "Map" [Lambda.LMonoTy.ftvar "k", Lambda.LMonoTy.ftvar "v"] ()))
    (Lambda.LExpr.bvar 0)
    (Lambda.LExpr.quant
      (Lambda.QuantifierKind.all)
@@ -301,8 +305,9 @@ info: [Lambda.LExpr.quant
                  u:select
                  (some (Lambda.LMonoTy.tcons
                     "arrow"
-                    [Lambda.LMonoTy.tcons "Map" [Lambda.LMonoTy.ftvar "k", Lambda.LMonoTy.ftvar "v"],
-                     Lambda.LMonoTy.tcons "arrow" [Lambda.LMonoTy.ftvar "k", Lambda.LMonoTy.ftvar "v"]])))
+                    [Lambda.LMonoTy.tcons "Map" [Lambda.LMonoTy.ftvar "k", Lambda.LMonoTy.ftvar "v"] (),
+                     Lambda.LMonoTy.tcons "arrow" [Lambda.LMonoTy.ftvar "k", Lambda.LMonoTy.ftvar "v"] ()]
+                    ())))
                (Lambda.LExpr.app
                  (Lambda.LExpr.app
                    (Lambda.LExpr.app
@@ -310,14 +315,17 @@ info: [Lambda.LExpr.quant
                        u:update
                        (some (Lambda.LMonoTy.tcons
                           "arrow"
-                          [Lambda.LMonoTy.tcons "Map" [Lambda.LMonoTy.ftvar "k", Lambda.LMonoTy.ftvar "v"],
+                          [Lambda.LMonoTy.tcons "Map" [Lambda.LMonoTy.ftvar "k", Lambda.LMonoTy.ftvar "v"] (),
                            Lambda.LMonoTy.tcons
                              "arrow"
                              [Lambda.LMonoTy.ftvar "k",
                               Lambda.LMonoTy.tcons
                                 "arrow"
                                 [Lambda.LMonoTy.ftvar "v",
-                                 Lambda.LMonoTy.tcons "Map" [Lambda.LMonoTy.ftvar "k", Lambda.LMonoTy.ftvar "v"]]]])))
+                                 Lambda.LMonoTy.tcons "Map" [Lambda.LMonoTy.ftvar "k", Lambda.LMonoTy.ftvar "v"] ()]
+                                ()]
+                             ()]
+                          ())))
                      (Lambda.LExpr.bvar 3))
                    (Lambda.LExpr.bvar 1))
                  (Lambda.LExpr.bvar 0)))
@@ -328,8 +336,9 @@ info: [Lambda.LExpr.quant
                  u:select
                  (some (Lambda.LMonoTy.tcons
                     "arrow"
-                    [Lambda.LMonoTy.tcons "Map" [Lambda.LMonoTy.ftvar "k", Lambda.LMonoTy.ftvar "v"],
-                     Lambda.LMonoTy.tcons "arrow" [Lambda.LMonoTy.ftvar "k", Lambda.LMonoTy.ftvar "v"]])))
+                    [Lambda.LMonoTy.tcons "Map" [Lambda.LMonoTy.ftvar "k", Lambda.LMonoTy.ftvar "v"] (),
+                     Lambda.LMonoTy.tcons "arrow" [Lambda.LMonoTy.ftvar "k", Lambda.LMonoTy.ftvar "v"] ()]
+                    ())))
                (Lambda.LExpr.bvar 3))
              (Lambda.LExpr.bvar 2))))))]
 -/
